stdlib/lampe/Stdlib/Slice.lean
@@ -20,32 +20,38 @@ lemma for_each_inv {T Env p f fb l}
     STHoare p env (Inv [] ⋆ [λf ↦ fb]) ((«std::slice::for_each».call h![T, Env] h![l, f])) (fun _ => Inv l ⋆ [λf ↦ fb]) := by
   enter_decl
   steps []
-  apply STHoare.letIn_intro (Q := fun _ => Inv l ⋆ [λf ↦ fb])
-  · apply STHoare.ramified_frame_top
-      (STHoare.loop_inv_intro' (Inv := fun i _ _ => Inv (l.take i) ⋆ [λf ↦ fb]) ?_)
-    · simp_all
-      simp [Nat.mod_eq_of_lt (by assumption)]
-      sl
-      simp
-    · intro i ihl ihg
-      steps
-      simp_all
-      casesm ∃_,_
-      have : i % 4294967296 = i := by
-        apply Nat.mod_eq_of_lt
-        apply lt_trans ihg
-        apply Nat.mod_lt
-        simp
-      apply STHoare.letIn_intro
-      · apply STHoare.callLambda_intro
-        apply h_inv (lp := l.take i)
-        simp_all [List.take_prefix]
-      · intro
-        steps allow_sl
-        simp_all
-        sl
-  intro
-  steps
+  loop_inv nat fun i _ _ => Inv (l.take i) ⋆ [λf ↦ fb]
+  · intro i ihl ihg
+    steps
+    casesm ∃_,_
+    subst_vars
+
+  -- apply STHoare.letIn_intro (Q := fun _ => Inv l ⋆ [λf ↦ fb])
+  -- · apply STHoare.ramified_frame_top
+  --     (STHoare.loop_inv_intro' (Inv := fun i _ _ => Inv (l.take i) ⋆ [λf ↦ fb]) ?_)
+  --   · simp_all
+  --     simp [Nat.mod_eq_of_lt (by assumption)]
+  --     sl
+  --     simp
+  --   · intro i ihl ihg
+  --     steps
+  --     simp_all
+  --     casesm ∃_,_
+  --     have : i % 4294967296 = i := by
+  --       apply Nat.mod_eq_of_lt
+  --       apply lt_trans ihg
+  --       apply Nat.mod_lt
+  --       simp
+  --     apply STHoare.letIn_intro
+  --     · apply STHoare.callLambda_intro
+  --       apply h_inv (lp := l.take i)
+  --       simp_all [List.take_prefix]
+  --     · intro
+  --       steps allow_sl
+  --       simp_all
+  --       sl
+  -- intro
+  -- steps
 
 lemma slice_map_inv {T U Env p f fb l}
     (Inv: List (Tp.denote p T) → List (Tp.denote p U) → SLP (State p))
@@ -56,6 +62,6 @@ lemma slice_pure_map {T U Env p f fb func l}
     (h_pure : ∀x, STHoare p env ⟦⟧ (fb h![x]) (fun r => r = func x)):
     STHoare p env [λf ↦ fb] ((«std::slice::map».call h![T, U, Env] h![l, f])) (fun v => v = l.map func) := by
   steps [slice_map_inv (Inv := fun i o => o = i.map func)]
-  · rfl
   · assumption
+  · rfl
   · intros; steps [h_pure]; simp_all
